Auto/Embedding/LamBase.lean
@@ -2566,7 +2566,7 @@ theorem LamTerm.maxLooseBVarSucc.spec (m : Nat) :
     rw [Nat.pred_succ] at IH'; exact IH'
   case mpr =>
     let h' := Nat.succ_le_succ h
-    apply IH.mpr; rw [Nat.succ_pred] at h'; exact h'
+    apply IH.mpr; rw [← Nat.pred_eq_sub_one, Nat.succ_pred] at h'; exact h'
     revert h; cases (maxLooseBVarSucc t)
     case zero => intro h; cases h
     case succ _ => intro _; simp
@@ -2954,7 +2954,7 @@ theorem LamTerm.getLamBodyN_mkLamFN_length_eq
     cases l <;> cases h
     case refl s' l =>
       dsimp [mkLamFN, getLamBodyN]
-      dsimp [Nat.add] at IH; apply IH; rfl
+      apply IH; rfl
 
 def LamTerm.getLamTysN (n : Nat) (t : LamTerm) : Option (List LamSort) :=
   match n with
@@ -3047,7 +3047,7 @@ theorem LamTerm.getAppArgsAux_eq : getAppArgsAux args t = getAppArgsAux [] t ++ 
     dsimp [getAppArgsAux]; rw [IHFn (args:=(s, arg) :: args), IHFn (args:=[(s, arg)])]
     rw [List.append_assoc]; rfl
 
-theorem LamTerm.maxEVarSucc_getAppArgsAux
+noncomputable def LamTerm.maxEVarSucc_getAppArgsAux
   (hs : HList (fun (_, arg) => arg.maxEVarSucc ≤ n) args) (ht : t.maxEVarSucc ≤ n) :
   HList (fun (_, arg) => arg.maxEVarSucc ≤ n) (LamTerm.getAppArgsAux args t) := by
   induction t generalizing args <;> try exact hs
@@ -3060,7 +3060,7 @@ def LamTerm.getAppArgs := getAppArgsAux []
 theorem LamTerm.getAppArgs_app : getAppArgs (.app s fn arg) = getAppArgs fn ++ [(s, arg)] := by
   dsimp [getAppArgs, getAppArgsAux]; rw [getAppArgsAux_eq]
 
-theorem LamTerm.maxEVarSucc_getAppArgs :
+noncomputable def LamTerm.maxEVarSucc_getAppArgs :
   HList (fun (_, arg) => arg.maxEVarSucc ≤ t.maxEVarSucc) (LamTerm.getAppArgs t) :=
   LamTerm.maxEVarSucc_getAppArgsAux .nil (Nat.le_refl _)
 
@@ -3117,7 +3117,7 @@ theorem LamTerm.getAppArgsNAux_eq : getAppArgsNAux n args t = (getAppArgsNAux n 
       cases getAppArgsNAux n [] fn <;> dsimp
       rw [List.append_assoc]; rfl
 
-theorem LamTerm.maxEVarSucc_getAppArgsNAux
+def LamTerm.maxEVarSucc_getAppArgsNAux
   (hs : HList (fun (_, arg) => arg.maxEVarSucc ≤ m) args) (ht : t.maxEVarSucc ≤ m)
   (heq : LamTerm.getAppArgsNAux n args t = .some args') :
   HList (fun (_, arg) => arg.maxEVarSucc ≤ m) args' := by
@@ -3131,7 +3131,7 @@ theorem LamTerm.maxEVarSucc_getAppArgsNAux
 
 def LamTerm.getAppArgsN n := getAppArgsNAux n []
 
-theorem LamTerm.maxEVarSucc_getAppArgsN
+def LamTerm.maxEVarSucc_getAppArgsN
   (heq : LamTerm.getAppArgsN n t = .some l) :
   HList (fun (_, arg) => arg.maxEVarSucc ≤ t.maxEVarSucc) l :=
   LamTerm.maxEVarSucc_getAppArgsNAux .nil (Nat.le_refl _) heq
@@ -3193,7 +3193,7 @@ theorem LamTerm.getAppFnN_bvarAppsRev_length_eq
     cases l <;> cases heq
     case refl s' l =>
       rw [getAppFnN_succ']; dsimp [bvarAppsRev]
-      dsimp [Nat.add] at IH; rw [IH rfl]; rfl
+      rw [IH rfl]; rfl
 
 def LamTerm.getForallEFBody (t : LamTerm) : LamTerm :=
   match t with
@@ -3920,7 +3920,7 @@ def LamWF.ofLamCheck? {ltv : LamTyVal} :
   | .some (LamSort.base _), _ => intro contra; cases contra
   | .none, _ => intro contra; cases contra
 
-theorem LamWF.ofNonemptyLamWF (H : Nonempty (LamWF ltv ⟨lctx, t, s⟩)) :
+def LamWF.ofNonemptyLamWF (H : Nonempty (LamWF ltv ⟨lctx, t, s⟩)) :
   LamWF ltv ⟨lctx, t, s⟩ := by
   cases h₁ : LamTerm.lamCheck? ltv lctx t
   case none =>
@@ -4125,7 +4125,7 @@ theorem LamWF.interp_eqForallEFN'
   case nil =>
     dsimp [mkForallEFN, interp]
     conv =>
-      enter [2]; rw [IsomType.eqForall HList.nil_IsomType.{u + 1, u + 1, 0}]
+      enter [2]; rw [IsomType.eqForall HList.nil_IsomType.{0, u + 1, 0}]
       rw [PUnit.eqForall]; unfold HList.nil_IsomType; dsimp
       dsimp [pushLCtxs, pushLCtxsDep, Nat.blt, Nat.ble]
     apply congrArg; apply interp_substWF
