Auto/Embedding/LamBitVec.lean
@@ -129,8 +129,9 @@ namespace BVLems
         rw [Nat.shiftRight_eq_div_pow]; apply (Nat.le_iff_div_eq_zero (Nat.two_pow_pos _)).mpr
         rw [Nat.pred_lt_iff_le (Nat.two_pow_pos _)]
         apply Nat.le_trans (Nat.sub_le _ _) (Nat.pow_le_pow_of_le_right (.step .refl) h)
-      apply eq_of_val_eq; rw [toNat_ofNatLt, hzero]
-      rw [toNat_neg, Int.mod_def', Int.emod]; dsimp; rw [Nat.zero_mod]
+      apply eq_of_val_eq; rw [toNat_ofNatLt, ← Nat.pred_eq_sub_one, hzero]
+      rw [toNat_neg, Int.mod_def', Int.emod];
+      dsimp only [Int.ofNat_eq_coe, Int.ofNat_emod, Int.natAbs_ofNat]; rw [Nat.zero_mod]
       rw [Int.subNatNat_of_sub_eq_zero ((Nat.sub_eq_zero_iff_le).mpr (Nat.two_pow_pos _))]
       rw [Int.toNat_ofNat, BitVec.toNat_ofNat]
       cases n <;> try rfl
