Auto/Translation/Lam2DAtomAsFVar.lean
@@ -129,7 +129,7 @@ def withHyps (hyps : Array Expr) : ExternM (Array FVarId) := do
   let mut ret := #[]
   for hyp in hyps do
     let name := "_exHyp" ++ (← mkFreshId).toString
-    let newFVarId ← withLocalDecl name .default hyp .default
+    let newFVarId ← withLocalDecl name.toName .default hyp .default
     ret := ret.push newFVarId
   return ret
 
